src/cnf/cnf.lean
@@ -1,6 +1,7 @@
 /-
-This file contains the definitions of the conjunctive normal form.
-Variables are general. 
+This file contains the definitions of formulas in conjunctive normal form.
+CNF is implemented as a list of clauses (see clause.lean).
+The variable type used in the formula is polymorphic.
 
 Authors: Cayden Codel, Jeremy Avigad, Marijn Heule
 Carnegie Mellon University
@@ -24,6 +25,12 @@ variables {V : Type u} [decidable_eq V] [inhabited V]
 /- Conjunctive normal form is a list of clauses joined by logical ANDs -/
 def cnf (V : Type u) := list (clause V)
 
+-- Note that the above definition allows for duplication of clauses (and
+-- permutations of clauses), whereas a set definition would not (assuming a
+-- set definition of clauses as well). However, lists allow for computable 
+-- functions to be defined on them, which is important for proving that
+-- encoding methods, which are computable, are equisatisfiable
+
 namespace cnf
 
 open literal
@@ -33,7 +40,7 @@ open function
 
 /-! # Instance properties -/
 
-instance : inhabited (cnf V) := ⟨[default (clause V)]⟩
+instance : inhabited (cnf V) := ⟨[arbitrary (clause V)]⟩
 instance : has_mem (clause V) (cnf V) := ⟨list.mem⟩
 instance : has_emptyc (cnf V) := ⟨list.nil⟩
 instance : has_union (cnf V) := ⟨list.union⟩
@@ -56,7 +63,9 @@ end
 
 /-! ### Evaluation under assignment -/
 
-/- The clauses of the CNF are joined by conjunctions, so all must evaluate to true -/
+-- Note: The below implementation works as well as a countp/filter, too
+/- The clauses of the CNF are joined by conjunctions, so for the evaluation
+   of a formula to be true, all clauses within must evaluate to true -/
 protected def eval (α : assignment V) (f : cnf V) : bool :=
   f.foldr (λ c b, b && (clause.eval α c)) tt
 
@@ -70,169 +79,142 @@ theorem eval_cons {α : assignment V} {c : clause V} {f : cnf V} :
   cnf.eval α (c :: f) = (clause.eval α c && cnf.eval α f) :=
 by simp only [cnf.eval, foldr, bool.band_comm]
 
-theorem ne_nil_of_eval_ff {α : assignment V} {f : cnf V} :
-  cnf.eval α f = ff → f ≠ [] :=
-by { contrapose, simp, intro h, simp [h] }
-
 theorem eval_ff_cons_of_eval_ff {α : assignment V} {f : cnf V} (c : clause V) :
   cnf.eval α f = ff → cnf.eval α (c :: f) = ff :=
-by { simp [cnf.eval], intro h, simp [h] }
+assume h, by rw [eval_cons, h, band_ff]
 
 theorem eval_append (α : assignment V) (f₁ f₂ : cnf V) : 
   cnf.eval α (f₁ ++ f₂) = cnf.eval α f₁ && cnf.eval α f₂ :=
-by { induction f₁ with c cs ih, simp, simp [eval_cons, ih] }
-
-lemma forall_clause_eval_tt_of_eval_tt {α : assignment V} {f : cnf V} : 
-  cnf.eval α f = tt → ∀ c ∈ f, clause.eval α c = tt :=
 begin
-  induction f with c cs ih,
-  { simp },
-  { simp [eval_cons], 
-    intros hc hcs,
-    exact and.intro hc (ih hcs) }
-end
-
-lemma eval_tt_of_forall_clause_eval_tt {α : assignment V} {f : cnf V} :
-  (∀ c ∈ f, clause.eval α c = tt) → cnf.eval α f = tt :=
-begin
-  induction f with c cs ih,
-  { simp },
-  { simp [eval_cons],
-    intros hc he,
-    simp [hc, ih he] }
+  unfold cnf.eval,
+  rw foldr_append,
+  cases foldr (λ c b, b && clause.eval α c) tt f₂,
+  { rw [band_ff, foldr_band_ff] },
+  { rw band_tt }
 end
 
 theorem eval_tt_iff_forall_clause_eval_tt {α : assignment V} {f : cnf V} :
   cnf.eval α f = tt ↔ ∀ c ∈ f, clause.eval α c = tt :=
-⟨forall_clause_eval_tt_of_eval_tt, eval_tt_of_forall_clause_eval_tt⟩
-
-lemma exists_clause_eval_ff_of_eval_ff {α : assignment V} {f : cnf V} : 
-  cnf.eval α f = ff → ∃ c ∈ f, clause.eval α c = ff :=
 begin
-  induction f with c cs ih,
-  { simp },
-  { simp [eval_cons], 
-    rintros (hc | hcs),
-    { use [c, hc] },
-    { rcases ih hcs with ⟨c, hc1, hc2⟩,
-      use c, simp [hc1, hc2] } },
-end
-
-lemma eval_ff_of_exists_clause_eval_ff {α : assignment V} {f : cnf V} :
-  (∃ c ∈ f, clause.eval α c = ff) → cnf.eval α f = ff :=
-begin
-  induction f with c cs ih,
-  { simp },
-  { rintros ⟨cl, hcl, heval⟩,
-    rcases eq_or_mem_of_mem_cons hcl with (rfl | h),
-    { simp only [eval_cons, heval, ff_band] },
-    { exact eval_ff_cons_of_eval_ff c (ih ⟨cl, h, heval⟩) } }
+  split,
+  { induction f with c cs ih,
+    { intros _ c hc, exact absurd hc (not_mem_nil _) },
+    { simp [eval_cons],
+      intros hc hcs,
+      exact and.intro hc (ih hcs) } },
+  { induction f with c cs ih,
+    { rw eval_nil, tautology },
+    { simp [eval_cons],
+      intros hc hcs,
+      exact and.intro hc (ih hcs) } }
 end
 
 theorem eval_ff_iff_exists_clause_eval_ff {α : assignment V} {f : cnf V} :
   cnf.eval α f = ff ↔ ∃ c ∈ f, clause.eval α c = ff :=
-⟨exists_clause_eval_ff_of_eval_ff, eval_ff_of_exists_clause_eval_ff⟩
+begin
+  split,
+  { induction f with c cs ih,
+    { rw eval_nil, contradiction },
+    { simp [eval_cons],
+      rintros (hc | hcs),
+      { use [c, hc] },
+      { rcases ih hcs with ⟨cl, hcl₁, hcl₂⟩,
+        use [cl, or.inr hcl₁, hcl₂] } } },
+  { induction f with c cs ih,
+    { rintros ⟨cl, hcl, _⟩, exact absurd hcl (not_mem_nil _) },
+    { rintros ⟨cl, hcl, heval⟩,
+      rcases eq_or_mem_of_mem_cons hcl with rfl | h,
+      { rw [eval_cons, heval, ff_band] },
+      { exact eval_ff_cons_of_eval_ff c (ih ⟨cl, h, heval⟩) } } }
+end
+
+theorem ne_nil_of_eval_ff {α : assignment V} {f : cnf V} :
+  f.eval α = ff → f ≠ [] :=
+begin
+  intro h,
+  rcases eval_ff_iff_exists_clause_eval_ff.mp h with ⟨cl, hcl, _⟩,
+  exact ne_nil_of_mem hcl
+end
 
 /-! ### Counting -/
 
 /- Counts the number of clauses which evaluate to true under some assignment -/
-def count_tt (α : assignment V) (f : cnf V) : nat :=
-  length $ f.filter (λ c, c.eval α = tt)
+protected def count_tt (α : assignment V) (f : cnf V) : nat :=
+  f.countp (λ c, clause.eval α c = tt)
 
 /- Counts the number of clauses which evaluate to false under some assignment -/
-def count_ff (α : assignment V) (f : cnf V) : nat :=
-  length $ f.filter (λ c, c.eval α = ff)
+protected def count_ff (α : assignment V) (f : cnf V) : nat :=
+  f.countp (λ c, clause.eval α c = ff)
 
-/-! ### Tseitin groundwork -/
+@[simp] theorem count_tt_nil (α : assignment V) : cnf.count_tt α [] = 0 := rfl
+@[simp] theorem count_ff_nil (α : assignment V) : cnf.count_ff α [] = 0 := rfl
 
--- A manual definition for vars using fold. Hard to prove things about
--- so the alternative definition is used
-/-
-def vars : cnf → list nat
-| []        := []
-| (c :: cs) := list.foldr (λ v s, if v ∈ s then s else v :: s) (vars cs) (clause.vars c)
--/
+/-! # vars -/
 
-protected def vars : cnf V → list V
-| []        := []
-| (c :: cs) := (vars cs) ∪ (clause.vars c) -- I prefer the union the other way, but alas...
+-- Extract the variables used in the clauses, as a set
+protected def vars : cnf V → finset V
+| []        := ∅
+| (c :: cs) := (c.vars) ∪ (vars cs)
 
-@[simp] theorem vars_nil : cnf.vars ([] : cnf V) = [] := rfl
+@[simp] theorem vars_nil : cnf.vars ([] : cnf V) = ∅ := rfl
 
 @[simp] theorem vars_singleton (c : clause V) : cnf.vars [c] = clause.vars c :=
-by simp [cnf.vars, var, nil_union]
+by { unfold cnf.vars, rw finset.union_empty }
 
-theorem vars_append_subset_union (f₁ f₂ : cnf V) :
-  cnf.vars (f₁ ++ f₂) ⊆ cnf.vars f₁ ∪ cnf.vars f₂ :=
+theorem mem_vars_cons_of_mem_vars {f : cnf V} {v : V} (c : clause V) :
+  v ∈ f.vars → v ∈ cnf.vars (c :: f) :=
+assume h, finset.mem_union.mpr (or.inr h)
+
+theorem clause_vars_subset_of_vars_of_mem {f : cnf V} {c : clause V} :
+  c ∈ f → (c.vars) ⊆ f.vars :=
 begin
-  sorry
+  induction f with cl cls ih,
+  { intro h, exact absurd h (not_mem_nil _) },
+  { intros hc v hv,
+    rcases eq_or_mem_of_mem_cons hc with rfl | hc,
+    { unfold cnf.vars,
+      rw finset.mem_union,
+      exact or.inl hv },
+    { exact mem_vars_cons_of_mem_vars cl (ih hc hv) } }
 end
 
-theorem vars_union_subset_append (f₁ f₂ : cnf V) :
-  cnf.vars f₁ ∪ cnf.vars f₂ ⊆ cnf.vars (f₁ ++ f₂) :=
+theorem exists_mem_clause_and_mem_of_mem_vars {f : cnf V} {v : V} :
+  v ∈ f.vars → ∃ (c : clause V), c ∈ f ∧ v ∈ c.vars :=
 begin
-  sorry
+  induction f with cl cls ih,
+  { rw vars_nil, intro h, exact absurd h (finset.not_mem_empty _) },
+  { intro hm,
+    by_cases h : (v ∈ cl.vars),
+    { use [cl, and.intro (mem_cons_self _ _) h] },
+    { unfold cnf.vars at hm,
+      rcases ih (or.resolve_left (finset.mem_union.mp hm) h) with ⟨c, hc, hcv⟩,
+      use [c, and.intro (mem_cons_of_mem cl hc) hcv] } }
 end
 
-theorem clause_vars_subset_of_mem {f : cnf V} {c : clause V} :
-  c ∈ f → (clause.vars c) ⊆ cnf.vars f :=
-begin
-  intro h,
-  induction f with d ds ih,
-  { exact absurd h (not_mem_nil c) },
-  { rcases eq_or_mem_of_mem_cons h with rfl | h2,
-    { simp [cnf.vars],
-      intros a ha,
-      exact mem_union_right (cnf.vars ds) ha },
-    { have ihred := ih h2,
-      unfold cnf.vars,
-      intros a ha,
-      exact mem_union_left (ihred ha) (d.vars) } }
-end
-
-theorem mem_vars_of_mem_clause_of_mem {f : cnf V} {c : clause V} {v : V} :
-  c ∈ f → v ∈ (clause.vars c) → v ∈ cnf.vars f :=
-begin
-  induction f with d ds ih,
-  { simp },
-  { intros hc hn,
-    rcases eq_or_mem_of_mem_cons hc with rfl | hds,
-    { simp [cnf.vars, hn] },
-    { simp [cnf.vars, ih hds hn] } }
-end
-
-protected theorem exists_mem_clause_of_mem_vars {f : cnf V} {v : V} :
-  v ∈ cnf.vars f → ∃ (c : clause V), c ∈ f ∧ v ∈ (clause.vars c) :=
-begin
-  induction f with c cs ih,
-  { simp },
-  { intro hn,
-    simp [cnf.vars] at hn,
-    rcases hn with hcs | hc,
-    { rcases ih hcs with ⟨cl, hcl, hcls⟩,
-      use cl,
-      simp [mem_cons_of_mem c hcl, hcls] },
-    { use c,
-      simp [mem_cons_self c cs, hc] } }
-end
-
-theorem subset_vars_of_subset_cnf {f₁ f₂ : cnf V} :
+theorem vars_subset_of_subset {f₁ f₂ : cnf V} :
   f₁ ⊆ f₂ → (cnf.vars f₁) ⊆ (cnf.vars f₂) :=
 begin
-  intros h n hn,
-  rcases cnf.exists_mem_clause_of_mem_vars hn with ⟨c, hf, hnc⟩,
-  exact mem_vars_of_mem_clause_of_mem (h hf) hnc
+  intros h v hv,
+  rcases cnf.exists_mem_clause_and_mem_of_mem_vars hv with ⟨c, hf, hvc⟩,
+  exact clause_vars_subset_of_vars_of_mem (h hf) hvc
 end
 
-theorem exists_not_mem_vars_of_bijection {g : V → nat} (hg : bijective g) (f : cnf V) :
-  ∃ (v : V), v ∉ cnf.vars f :=
+-- It is important to produce a variable not in the vars of a formula
+-- We produce the variable as the successor of the largest variable,
+-- if given a bijection between the variable type and the natural numbers
+
+-- TODO: Maybe refine this theorem/definition with something else in lib.
+theorem exists_not_mem_vars_of_bijection {g : V → nat} (f : cnf V) : 
+  bijective g → ∃ (v : V), v ∉ cnf.vars f :=
 begin
+  intro hg,
   cases f,
-  { use [(arbitrary V), not_mem_nil _] },
-  { have : foldr max 0 (map g (cnf.vars (f_hd :: f_tl))) + 1 > 
-      foldr max 0 (map g (cnf.vars (f_hd :: f_tl))),
+  { use [(arbitrary V), finset.not_mem_empty _] },
+  { have : (max_nat (map g (cnf.vars (f_hd :: f_tl)).to_list)) + 1 > 
+      (max_nat (map g (cnf.vars (f_hd :: f_tl)).to_list)),
       from lt_add_one _,
-    rcases exists_not_mem_of_gt_max hg this with ⟨v, heq, hv⟩,
+    rcases exists_not_mem_of_bijective_of_gt_max_nat hg this with ⟨v, heq, hv⟩,
+    rw finset.mem_to_list at hv,
     use [v, hv] }
 end
 
@@ -241,37 +223,29 @@ theorem exists_not_mem_forall_clause_of_bijection
   {g : V → nat} (hg : bijective g) (f : cnf V) :
   ∃ (v : V), ∀ (c : clause V), c ∈ f → v ∉ clause.vars c :=
 begin
-  rcases exists_not_mem_vars_of_bijection hg f with ⟨v, hv⟩,
+  rcases exists_not_mem_vars_of_bijection f hg with ⟨v, hv⟩,
   use v,
   intros c hc hvnot,
-  have := clause_vars_subset_of_mem hc,
-  exact hv (this hvnot)
+  exact hv ((clause_vars_subset_of_vars_of_mem hc) hvnot)
 end
 
 /-! # Equisatisfiability -/
 
 def equisatisfiable (f₁ f₂ : cnf V) :=
-  (∃ (α₁ : assignment V), cnf.eval α₁ f₁ = tt) ↔ ∃ (α₂ : assignment V), cnf.eval α₂ f₂ = tt
+  (∃ (α₁ : assignment V), cnf.eval α₁ f₁ = tt) ↔ 
+   ∃ (α₂ : assignment V), cnf.eval α₂ f₂ = tt
 
 notation f₁ ` ≈ ` f₂ := equisatisfiable f₁ f₂
 
 @[simp] theorem equisatisfiable_nil : equisatisfiable ([] : cnf V) [] :=
-by simp [equisatisfiable]
+⟨λ h, h, λ h, h⟩
 
 @[refl] theorem equisatisfiable.refl (f : cnf V) : f ≈ f :=
-begin
-  split;
-  { rintros ⟨α, ha⟩,
-    use [α, ha] }
-end
+⟨λ h, h, λ h, h⟩
 
 @[symm] theorem equisatisfiable.symm (f₁ f₂ : cnf V) :
   f₁ ≈ f₂ → f₂ ≈ f₁ :=
-begin
-  unfold equisatisfiable,
-  rintros ⟨hmp, hmpr⟩,
-  exact ⟨hmpr, hmp⟩
-end
+assume h, ⟨h.2, h.1⟩
 
 @[trans] theorem equisatisfiable.trans {f₁ f₂ f₃ : cnf V} :
   f₁ ≈ f₂ → f₂ ≈ f₃ → f₁ ≈ f₃ :=
@@ -281,13 +255,6 @@ begin
   { intro h, exact hmp2 (hmp1 h) },
   { intro h, exact hmpr1 (hmpr2 h) }
 end
-
--- Can make this be an equivalence relation now
-
-/-! # Equivalence -/
-
-def equivalent (f₁ f₂ : cnf V) :=
-  ∀ (α : assignment V), cnf.eval α f₁ = cnf.eval α f₂
 
 end cnf
 
@@ -300,21 +267,21 @@ open clause
 open cnf
 open list
 
-theorem eval_eq_of_equiv_on_domain_vars {α₁ α₂ : assignment V} {f : cnf V} :
-  (α₁ ≡[f.vars]≡ α₂) → cnf.eval α₁ f = cnf.eval α₂ f :=
+theorem eval_eq_cnf_of_eqod {α₁ α₂ : assignment V} {f : cnf V} :
+  (α₁ ≡f.vars≡ α₂) → f.eval α₁ = f.eval α₂ :=
 begin
   intro h,
-  cases he : (cnf.eval α₂ f),
+  cases hev : (cnf.eval α₂ f),
   { apply eval_ff_iff_exists_clause_eval_ff.mpr,
-    rcases eval_ff_iff_exists_clause_eval_ff.mp he with ⟨c, hc, hff⟩,
+    rcases eval_ff_iff_exists_clause_eval_ff.mp hev with ⟨c, hc, hff⟩,
     use [c, hc],
-    exact eval_eq_of_equiv_on_clause2 
-      (eqod_subset_of_eqod (clause_vars_subset_of_mem hc) h).symm ▸ hff },
+    exact hff ▸ eval_eq_clause_of_eqod 
+      (eqod_subset (clause_vars_subset_of_vars_of_mem hc) h) },
   { apply eval_tt_iff_forall_clause_eval_tt.mpr,
     intros c hc,
-    exact (eval_eq_of_equiv_on_clause2
-      (eqod_subset_of_eqod (clause_vars_subset_of_mem hc) h)).symm ▸
-      (eval_tt_iff_forall_clause_eval_tt.mp he c hc) }
+    have := eval_tt_iff_forall_clause_eval_tt.mp hev c hc,
+    exact this ▸ eval_eq_clause_of_eqod
+      (eqod_subset (clause_vars_subset_of_vars_of_mem hc) h) }
 end
 
 end assignment
