src/cnf/explode.lean
@@ -3,8 +3,6 @@ This file contains the definition of the "explode" operation, which
 creates a "powerset" of literals from a list of variables. Associated
 theorems dealing with the contents of explode are also included.
 
-Variables are general.
-
 Authors: Cayden Codel, Jeremy Avigad, Marijn Heule
 Carnegie Mellon University
 -/
@@ -26,195 +24,188 @@ open clause
 open list
 open function
 
-/- Sometimes, it is necessary to get all possible disjunctive clauses from a set of variables -/
-/- For lack of a better name, we call that operation "exploding" -/
-
--- NOTE: If clauses are switched to sets, explode may also be appropriate as a (fin)set
+/- Sometimes, it is necessary to take a list of variables and produce a list
+   of all possible positive and negative forms of those variables, maintaining
+   the order of the original list. We call this operation, "exploding." -/
 
 namespace explode
+
+variables {v : V} {l : list V} {c : clause V}
 
 /-! # Explode -/
 
 def explode : list V → list (clause V)
 | []        := [[]]
-| (v :: vs) := (explode vs).map (cons (Pos v)) ++ (explode vs).map (cons (Neg v))
+| (v :: l) := (explode l).map (cons (Pos v)) ++ (explode l).map (cons (Neg v))
 
 @[simp] theorem explode_nil : explode ([] : list V) = [[]] := rfl
 
 @[simp] theorem explode_singleton (v : V) : explode [v] = [[Pos v], [Neg v]] :=
-by simp [explode]
+by refl
 
-theorem length_explode : ∀ (l : list V), length (explode l) = 2^(length l)
-| []        := rfl
-| (v :: vs) := by simp [explode, length_explode vs, pow_succ, two_mul]
+theorem length_explode (l : list V) : length (explode l) = 2^(length l) :=
+begin
+  induction l with v vs ih,
+  { refl },
+  { simp only [explode, length_cons, length_append, 
+      length_map, pow_succ, two_mul, ih] }
+end
 
 theorem length_explode_pos (l : list V) : length (explode l) > 0 :=
-by simp [length_explode]
+by { rw length_explode, exact pow_pos zero_lt_two _ }
 
 theorem exists_mem_explode (l : list V) : ∃ (c : clause V), c ∈ explode l :=
 exists_mem_of_length_pos (length_explode_pos _)
 
-theorem length_eq_of_mem_explode {l : list V} : 
-  ∀ {c : clause V}, c ∈ explode l → length c = length l :=
+theorem length_eq_of_mem_explode : c ∈ explode l → length c = length l :=
 begin
-  induction l with n ns ih, { simp },
+  induction l with v vs ih generalizing c,
+  { rw [explode_nil, mem_singleton], 
+    rintro rfl, refl },
   { simp only [explode, mem_append, mem_map],
-    rintros c (⟨c, hc, rfl⟩ | ⟨c, hc, rfl⟩); simp [length, ih hc] }
+    rintros (⟨c, hc, rfl⟩ | ⟨c, hc, rfl⟩);
+    { simp [ih hc, length_cons] } }
 end
 
-theorem mem_explode_cons_of_mem_explode_of_lit {l : list V} (lit : literal V) : 
-  ∀ {c : clause V}, c ∈ explode l → (lit :: c) ∈ explode (lit.var :: l) :=
-assume c hc, by { cases lit; simp [explode, literal.var, hc] }
+theorem cons_mem_explode_cons_of_mem_explode (lit : literal V) : 
+  c ∈ explode l → (lit :: c) ∈ explode (lit.var :: l) :=
+assume hc, by { cases lit; simp [explode, literal.var, hc] }
 
-lemma map_var_eq_of_mem_explode {l : list V} : 
-  ∀ {c : clause V}, c ∈ explode l → map var c = l :=
+theorem mem_of_mem_explode_of_mem_vars : 
+  c ∈ explode l → v ∈ c.vars → v ∈ l :=
 begin
-  induction l with n ns ih,
-  { simp },
+  induction l with v vs ih generalizing c,
+  { rw [explode_nil, mem_singleton],
+    rintros rfl hv, 
+    rw clause.vars_nil at hv,
+    exact absurd hv (finset.not_mem_empty _) },
   { simp only [explode, mem_append, mem_map],
-    rintros c (⟨a, ha, rfl⟩ | ⟨a, ha, rfl⟩);
-    { simp [var, map_cons, ih ha] } }
+    rintros (⟨a, ha, rfl⟩ | ⟨a, ha, rfl⟩);
+    { intros hv,
+      unfold clause.vars at hv,
+      rw finset.mem_union at hv,
+      rw mem_cons_iff,
+      rcases hv with hv | hv,
+      { unfold var at hv,
+        rw finset.mem_singleton at hv,
+        exact or.inl hv },
+      { exact or.inr (ih ha hv) } } }
 end
 
-lemma mem_explode_of_map_var_eq {l : list V} : 
-  ∀ {c : clause V}, c.map var = l → c ∈ explode l :=
+theorem mem_vars_of_mem_explode_of_mem :
+  c ∈ explode l → v ∈ l → v ∈ c.vars :=
 begin
-  induction l with n ns ih,
-  { simp },
-  { intros c h,
-    rcases exists_cons_of_map_cons h with ⟨l, ls, rfl, hl, hls⟩,
-    rcases pos_or_neg_of_var_eq_nat hl with rfl | rfl,
-    { simp [explode], left, use ls, simp [ih hls] },
-    { simp [explode], right, use ls, simp [ih hls] } }
+  induction l with v vs ih generalizing c,
+  { intros _ hv, exact absurd hv (not_mem_nil v) } ,
+  { simp only [explode, mem_append, mem_map],
+    rintros (⟨a, ha, rfl⟩ | ⟨a, ha, rfl⟩) hv;
+    { unfold clause.vars var,
+      rcases eq_or_mem_of_mem_cons hv with rfl | hv,
+      { exact finset.mem_union.mpr (or.inl (mem_singleton_self _)) },
+      { exact finset.mem_union.mpr (or.inr (ih ha hv)) } } }
 end
-
-theorem mem_explode_iff_map_var_eq {l : list V} {c : clause V} : 
-  c.map var = l ↔ c ∈ explode l :=
-⟨mem_explode_of_map_var_eq, map_var_eq_of_mem_explode⟩
-
--- Some way of compressing casework into a "repeat"?
--- TODO think about pulling c, c ∈ explode into hypotheses to remove "of_mem_explode"
-lemma mem_clause_of_mem_of_mem_explode {l : list V} : 
-  ∀ {c : clause V}, c ∈ explode l → ∀ {v : V}, v ∈ l → Pos v ∈ c ∨ Neg v ∈ c :=
-begin
-  induction l with m ms ih,
-  { simp },
-  simp only [explode, mem_append, mem_map],
-  rintros c (⟨d, hd, rfl⟩ | ⟨d, hd, rfl⟩) n (rfl | hn),
-  { simp [mem_cons_self] },
-  { cases ih hd hn with h h; 
-    simp [mem_cons_of_mem _ h] },
-  { simp [mem_cons_self] },
-  { cases ih hd hn with h h; 
-    simp [mem_cons_of_mem _ h] }
-end
-
--- Reduce casework?
-lemma mem_of_mem_clause_of_mem_explode {l : list V} :
-  ∀ {c : clause V}, c ∈ explode l → ∀ {v : V}, Pos v ∈ c ∨ Neg v ∈ c → v ∈ l :=
-begin
-  induction l with m ms ih,
-  { simp },
-  simp only [explode, mem_append, mem_map],
-  rintros c (⟨a, ha, rfl⟩ | ⟨a, ha, rfl⟩) n (hn | hn),
-  { rcases eq_or_mem_of_mem_cons hn with (hn₁ | hn₂),
-    { have := congr_arg literal.var hn₁,
-      simp [var] at this,
-      simp [this] },
-    { exact mem_cons_of_mem _ (ih ha (or.inl hn₂)) } },
-  { rcases eq_or_mem_of_mem_cons hn with (hn₁ | hn₂),
-    { have := congr_arg literal.var hn₁,
-      simp [var] at this,
-      simp [this] },
-    { exact mem_cons_of_mem _ (ih ha (or.inr hn₂)) } },
-  { rcases eq_or_mem_of_mem_cons hn with (hn₁ | hn₂),
-    { have := congr_arg literal.var hn₁,
-      simp [var] at this,
-      simp [this] },
-    { exact mem_cons_of_mem _ (ih ha (or.inl hn₂)) } },
-  { rcases eq_or_mem_of_mem_cons hn with (hn₁ | hn₂),
-    { have := congr_arg literal.var hn₁,
-      simp [var] at this,
-      simp [this] },
-    { exact mem_cons_of_mem _ (ih ha (or.inr hn₂)) } }
-end
-
-theorem mem_iff_mem_clause_of_mem_explode {l : list V} :
-  ∀ {c : clause V}, c ∈ explode l → ∀ {v : V}, Pos v ∈ c ∨ Neg v ∈ c ↔ v ∈ l :=
-assume c hc n, ⟨mem_of_mem_clause_of_mem_explode hc, 
-                mem_clause_of_mem_of_mem_explode hc⟩
 
 -- Corollaries of the above
-theorem mem_var_of_mem_clause_of_mem_explode {l : list V} :
-  ∀ {c : clause V}, c ∈ explode l → ∀ {lit : literal V}, lit ∈ c → literal.var lit ∈ l :=
+theorem not_mem_vars_of_mem_explode_of_not_mem :
+  c ∈ explode l → v ∉ l → v ∉ c.vars :=
 begin
-  intros c hc lit hl,
-  cases lit,
-  { simp [var, mem_of_mem_clause_of_mem_explode hc (or.inl hl)] },
-  { simp [var, mem_of_mem_clause_of_mem_explode hc (or.inr hl)] }
+  intro h,
+  contrapose,
+  simp only [not_not],
+  exact mem_of_mem_explode_of_mem_vars h
 end
 
-theorem not_mem_clause_of_not_mem_of_mem_explode {l : list V} : 
-  ∀ {c : clause V}, c ∈ explode l → ∀ {v : V}, v ∉ l → Pos v ∉ c ∧ Neg v ∉ c :=
+theorem not_mem_of_mem_explode_of_not_mem_vars :
+  c ∈ explode l → v ∉ c.vars → v ∉ l :=
 begin
-  intros c hc n,
+  intro h,
   contrapose,
-  simp [not_and_distrib],
-  exact mem_of_mem_clause_of_mem_explode hc
+  simp only [not_not],
+  exact mem_vars_of_mem_explode_of_mem h
 end
 
-theorem not_mem_of_not_mem_clause_of_mem_explode {l : list V} : 
-  ∀ {c : clause V}, c ∈ explode l → ∀ {v : V}, (Pos v ∉ c) ∧ (Neg v ∉ c) → v ∉ l :=
+theorem pos_or_neg_of_mem_explode_of_mem :
+  c ∈ explode l → v ∈ l → Pos v ∈ c ∨ Neg v ∈ c :=
+assume h hv, mem_vars_iff_pos_or_neg_mem_clause.mp 
+  (mem_vars_of_mem_explode_of_mem h hv)
+
+theorem pos_and_neg_not_mem_of_mem_explode_of_not_mem :
+  c ∈ explode l → v ∉ l → Pos v ∉ c ∧ Neg v ∉ c :=
 begin
-  intros c hc n,
+  intro h,
   contrapose,
-  simp [not_and_distrib],
-  exact mem_clause_of_mem_of_mem_explode hc
+  rw not_and_distrib,
+  simp only [not_not],
+  intro hv,
+  exact mem_of_mem_explode_of_mem_vars h 
+    (mem_vars_iff_pos_or_neg_mem_clause.mpr hv)
+end
+
+-- A theorems concerning the variables of input
+-- If explode changes type to (fin)set, remove/update theorem
+theorem map_var_eq_iff_mem_explode : c.map var = l ↔ c ∈ explode l :=
+begin
+  split,
+  { induction l with v vs ih generalizing c,
+    { simp only [explode_nil, imp_self, map_eq_nil, mem_singleton] },
+    { intro h,
+      rcases exists_cons_of_map_cons h with ⟨l, ls, rfl, hl, hls⟩,
+      rcases pos_or_neg_of_var_eq_nat hl with rfl | rfl,
+      { simp [explode], left, use [ls, ih hls] },
+      { simp [explode], right, use [ls, ih hls] } } },
+  { induction l with v vs ih generalizing c,
+    { simp only [explode_nil, imp_self, map_eq_nil, mem_singleton] },
+    { simp only [explode, mem_map, mem_append],
+      rintros (⟨a, ha, rfl⟩ | ⟨a, ha, rfl⟩);
+      { simp only [ih ha, var, map, eq_self_iff_true, and_self] } } }
 end
 
 /-! # nodup properties of explode -/
+-- Note: These are not necessary if nodup becomes a (fin)set
 
 theorem explode_nodup (l : list V) : nodup (explode l) :=
 begin
-  induction l with n ns ih,
-  { simp },
-  { simp [explode, nodup_cons],
-    apply nodup_append.mpr,
-    simp [nodup_map (cons_injective) ih],
-    intros x hx hxn,
-    rcases mem_map.mp hx with ⟨c, hc, hcx⟩,
-    rcases mem_map.mp hxn with ⟨d, hd, hdx⟩,
-    rw ← hcx at hdx,
-    exact absurd (head_eq_of_cons_eq hdx).symm (pos_ne_neg n) }
+  induction l with v vs ih,
+  { rw explode_nil, exact nodup_singleton nil },
+  { simp only [explode, nodup_cons, nodup_append],
+    simp only [nodup_map (cons_injective) ih, true_and],
+    intros x hxp hxn,
+    rcases mem_map.mp hxp with ⟨c, _, hcx⟩,
+    rcases mem_map.mp hxn with ⟨d, _, rfl⟩,
+    have := (head_eq_of_cons_eq hcx).symm,
+    contradiction }
 end
 
--- This can be made into a non-induction argument
-theorem mem_nodup_of_nodup {l : list V} (h : nodup l) :
-  ∀ {c : clause V}, c ∈ explode l → nodup c :=
+-- TODO Use simp to reduce?
+theorem nodup_of_nodup_of_mem (h : nodup l) : c ∈ explode l → nodup c :=
 begin
-  induction l with n ns ih,
-  { simp },
-  { intros c hc,
-    simp [explode] at hc,
-    rcases hc with ⟨a, ha, rfl⟩ | ⟨a, ha, rfl⟩;
-    { rcases not_mem_clause_of_not_mem_of_mem_explode 
-        ha (not_mem_of_nodup_cons h) with ⟨hpos, hneg⟩,
-      simp [hpos, hneg, ih (nodup_of_nodup_cons h) ha] } }
+  induction l with n ns ih generalizing c,
+  { rw [explode_nil, mem_singleton], rintro rfl, exact nodup_nil },
+  { intro hc,
+    simp only [explode, mem_append, mem_map] at hc,
+    rcases hc with ⟨a, ha, rfl⟩ | ⟨a, ha, rfl⟩,
+    { rw nodup_cons,
+      have := not_mem_of_nodup_cons h,
+      have := pos_and_neg_not_mem_of_mem_explode_of_not_mem ha this,
+      exact ⟨this.1, ih (nodup_of_nodup_cons h) ha⟩ },
+    { rw nodup_cons,
+      have := not_mem_of_nodup_cons h,
+      have := pos_and_neg_not_mem_of_mem_explode_of_not_mem ha this,
+      exact ⟨this.2, ih (nodup_of_nodup_cons h) ha⟩ } }
 end
 
-theorem xor_mem_clause_of_mem_of_mem_explode {l : list V} (h : nodup l) :
-  ∀ {c : clause V}, c ∈ explode l → ∀ {v : V}, v ∈ l → xor (Pos v ∈ c) (Neg v ∈ c) :=
+theorem xor_pos_neg_mem_clause_of_nodup_of_mem_explode_of_mem (h : nodup l) :
+  c ∈ explode l → v ∈ l → xor (Pos v ∈ c) (Neg v ∈ c) :=
 begin
-  induction l with m ms ih,
-  { simp },
-  { intros c hc n hn,
-    simp [explode] at hc,
-    rcases hc with ⟨a, ha, rfl⟩ | ⟨a, ha, rfl⟩;
-    { rcases eq_or_mem_of_mem_cons hn with (rfl | hn),
-      { simp [mem_cons_self, 
-        not_mem_clause_of_not_mem_of_mem_explode ha (not_mem_of_nodup_cons h)] },
-      { rcases ih (nodup_of_nodup_cons h) ha hn with ⟨hpos, hneg⟩ | ⟨hpos, hneg⟩;
-        { simp [hpos, hneg, ne_of_mem_of_not_mem hn (not_mem_of_nodup_cons h)] } } } }
+  induction l with v vs ih generalizing c,
+  { intros _ h, exact absurd h (not_mem_nil _) },
+  { simp only [explode, mem_append, mem_map],
+    rintros (⟨a, ha, rfl⟩ | ⟨a, ha, rfl⟩) hc;
+    { rcases eq_or_mem_of_mem_cons hc with (rfl | hv),
+      { simp [pos_and_neg_not_mem_of_mem_explode_of_not_mem ha 
+            (not_mem_of_nodup_cons h)] },
+      { rcases ih (nodup_of_nodup_cons h) ha hv with ⟨hp, hn⟩ | ⟨hp, hn⟩;
+        { simp [hp, hn, ne_of_mem_of_not_mem hv (not_mem_of_nodup_cons h)] } } } }
 end
 
 end explode
