src/basic.lean
@@ -1,18 +1,15 @@
 /-
+Some basic facts unrelated to clauses, etc.
 
-  Some basic facts unrelated to literals, clauses, etc. that are useful for proofs.
-
-  Author: Cayden Codel
-  Carnegie Mellon University
-
+Author: Cayden Codel, Marijn Heule, Jeremy Avigad
+Carnegie Mellon University
 -/
 
-import data.bool
+import data.bool.basic
 import data.list.basic
-import data.list.nodup
 import init.data.nat.lemmas
-import tactic
-
+import data.finset.basic
+import data.finset.fold
 import init.function
 
 open list
@@ -21,267 +18,61 @@ open function
 universes u v
 variables {α : Type u} {β : Type v}
 
--- Define shorthand for XOR
+/-! # Boolean logic -/
+
+/- bxor -/
+
 notation a ` ⊕ ` b := bxor a b
 
--- Some trivial, useful theorems
-@[simp] theorem bxor_tt_left  : ∀ a, bxor tt a = bnot a := dec_trivial
-@[simp] theorem bxor_tt_right : ∀ a, bxor a tt = bnot a := dec_trivial
+@[simp] theorem bxor_tt_left  : ∀ a, tt ⊕ a = !a := dec_trivial
+@[simp] theorem bxor_tt_right : ∀ a, a ⊕ tt = !a := dec_trivial
+
+theorem bxor_conjunctive (a b : bool) : a ⊕ b = (a || b) && (!a || !b) :=
+by cases a; cases b; dec_trivial
+
+theorem bxor_disjunctive (a b : bool) : a ⊕ b = (!a && b) || (a && !b) :=
+by cases a; cases b; dec_trivial
+
+/- cond -/
 
 @[simp] theorem cond_tt_ff : ∀ a, cond a tt ff = a := dec_trivial
-@[simp] theorem cond_ff_tt : ∀ a, cond a ff tt = bnot a := dec_trivial
+@[simp] theorem cond_ff_tt : ∀ a, cond a ff tt = !a := dec_trivial
 
 theorem tt_of_cond_ne_second [decidable_eq α] {c d : α} {b : bool} :
   cond b c d ≠ d → b = tt :=
-by cases b; simp
+by { cases b, contradiction, tautology }
 
 theorem ff_of_cond_ne_first [decidable_eq α] {c d : α} {b : bool} :
   cond b c d ≠ c → b = ff :=
-by cases b; simp
+by { cases b, tautology, contradiction }
 
-theorem tt_of_cond_eq_of_ne_second [decidable_eq α] {c d e : α} {b : bool} :
+theorem tt_of_ne_second_of_cond_eq [decidable_eq α] {c d e : α} {b : bool} :
   d ≠ e → cond b c d = e → b = tt :=
-begin
-  cases b,
-  { simp, exact id },
-  { tautology }
-end
+by { cases b, { intros, contradiction }, { tautology } }
 
-theorem ff_of_cond_eq_of_ne_first [decidable_eq α] {c d e : α} {b : bool} :
+theorem ff_of_ne_first_of_cond_eq [decidable_eq α] {c d e : α} {b : bool} :
   c ≠ e → cond b c d = e → b = ff :=
-begin
-  cases b,
-  { tautology },
-  { simp, exact id }
-end
+by { cases b, { tautology }, { intros, contradiction } }
 
-theorem band_tt_of_and_tt {b₁ b₂ : bool} : b₁ = tt ∧ b₂ = tt → b₁ && b₂ = tt :=
-begin
-  rintros ⟨h₁, h₂⟩,
-  simp [h₁, h₂]
-end
+theorem tt_of_ne_of_cond_eq_first [decidable_eq α] {c d : α} {b : bool} :
+  c ≠ d → cond b c d = c → b = tt :=
+by { cases b, { intros h₁ h₂, exact absurd h₂.symm h₁ }, { tautology } }
 
--- Expand xor in terms of other boolean operations
--- (Proof seems inane - shorten?)
-theorem bxor_conjunctive : ∀ (a b : bool), bxor a b = (a || b) && (!a || !b)
-| tt tt := dec_trivial
-| tt ff := dec_trivial
-| ff tt := dec_trivial
-| ff ff := dec_trivial
+theorem ff_of_ne_of_cond_eq_second [decidable_eq α] {c d : α} {b : bool} :
+  c ≠ d → cond b c d = d → b = ff :=
+by { cases b, { tautology }, { intros, contradiction }}
 
-theorem bxor_disjunctive : ∀ (a b : bool), bxor a b = (!a && b) || (a && !b)
-| tt tt := dec_trivial
-| tt ff := dec_trivial
-| ff tt := dec_trivial
-| ff ff := dec_trivial
+/-! # List operations -/
 
-theorem neq_of_ff_of_tt {a b : bool} : a = tt → b = ff → a ≠ b :=
-begin
-  intros ha hb, simp [ha, hb]
-end
+/- General results -/
 
-/- This is a shorthand for absurd that derives from a boolean that is true and false -/
-theorem absurd_bool {a : bool} {b : Prop} : a = tt → a = ff → b :=
-assume h₁ h₂, absurd h₁ (neq_of_ff_of_tt rfl h₂).symm
-
-/- Reasoning about cond is helpful if the result of the cond is known -/
-theorem cond_tt_of_cond_eq_first_of_ne [decidable_eq α] {a₁ a₂ : α} (b : bool) : 
-  a₂ ≠ a₂ → cond b a₁ a₂ = a₁ → b = tt :=
-by cases b; simp [imp_false]
-
-theorem cond_ff_of_cond_eq_second_of_ne [decidable_eq α] {a₁ a₂ : α} (b : bool) :
-  a₁ ≠ a₂ → cond b a₁ a₂ = a₂ → b = ff :=
-by cases b; simp [imp_false]
-
-theorem cond_tt_of_not_cond_eq_second_of_ne [decidable_eq α] {a₁ a₂ : α} (b : bool) :
-  a₁ ≠ a₂ → ¬(cond b a₁ a₂ = a₂) → b = tt :=
-by cases b; simp
-
-theorem cond_ff_of_not_cond_eq_first_of_ne [decidable_eq α] {a₁ a₂ : α} (b : bool) :
-  a₂ ≠ a₁ → ¬(cond b a₁ a₂ = a₁) → b = ff :=
-by cases b; simp
-
-theorem ne_tail_of_eq_head_of_ne [decidable_eq α] {a b : α} : ∀ {l₁ : list α},
-  ∀ {l₂ : list α}, (a :: l₁) ≠ (b :: l₂) → a = b → l₁ ≠ l₂
-| []        := by simp
-| (x :: xs) := begin
-  intros l₂ hneq heq,
-  by_contradiction,
-  exact absurd (congr (congr_arg cons heq) h) hneq
-end
-
--- Some facts about map that help
-theorem exists_of_map_singleton {f : α → β} {b : β} :
-  ∀ {l : list α}, map f l = [b] → ∃ a, [a] = l ∧ f a = b
-| []        := by { contradiction }
-| [x]       := by { simp [map_cons] }
-| (x :: y :: ys) := by { simp }
-
-theorem exists_cons_of_map_cons {f : α → β} {b : β} {bs : list β} :
-  ∀ {l : list α}, map f l = b :: bs → ∃ h L, l = h :: L ∧ f h = b ∧ map f L = bs
-| []        := by { contradiction }
-| (x :: xs) := begin 
-  simp [map_cons],
-  intros hx hxs,
-  use x, use xs, simp [hx, hxs]
-end
-
--- If instead the list from above is a map construction too
-theorem exists_map_cons_of_map_cons {f : α → β} {a : α} {as : list α} :
-  ∀ {l : list α}, map f l = map f (a :: as) → ∃ h L, l = h :: L ∧ f h = f a ∧ map f L = map f as
-| []        := by { contradiction }
-| (x :: xs) := begin
-  simp [map_cons],
-  intros hx hxs,
-  use [x, xs], simp [hx, hxs]
-end
-
-theorem mem_map_append {l₁ l₂ : list α} {f : α → β} {b : β} :
-  b ∈ map f (l₁ ++ l₂) → b ∈ map f l₁ ∨ b ∈ map f l₂ :=
-by simp
-
--- Or facts about filter
-theorem length_filter {p : α → Prop} [decidable_pred p] {l : list α} : 
-  length (filter p l) ≤ length l :=
-begin
-  induction l with x xs ih,
-  { simp },
-  { by_cases p x,
-    { simp [filter_cons_of_pos _ h, ih] },
-    { simp [filter_cons_of_neg _ h, ih, le_add_right] } }
-end
-
--- Sublists need membership theorems, too
-theorem mem_of_mem_sublist {l₁ l₂ : list α} {a : α} :
-  a ∈ l₁ → l₁ <+ l₂ → a ∈ l₂ :=
-assume ha hl, sublist.subset hl ha
-
-theorem not_mem_of_sublist_of_not_mem {l₁ l₂ : list α} {a : α} :
-  a ∉ l₂ → l₁ <+ l₂ → a ∉ l₁ :=
-assume ha hl h, absurd ((sublist.subset hl) h) ha
-
--- Very sad theorems on nats
-def max_nat : list nat → nat
-| []        := 0
-| (n :: ns) := max n (max_nat ns)
-
-theorem max_nat_is_max (l : list nat) : ∀ (n : nat), n ∈ l → n ≤ max_nat l :=
-begin
-  induction l with m ms ih,
-  { simp },
-  { intros n hn,
-    rcases eq_or_mem_of_mem_cons hn with rfl | hms,
-    { simp [max_nat] },
-    { simp [ih n hms, max_nat] } }
-end
-
-theorem not_mem_of_gt_max_nat {l : list nat} {n : nat} : n > max_nat l → n ∉ l :=
-begin
-  contrapose, simp, exact max_nat_is_max l n
-end
-
-theorem not_mem_of_gt_max {l : list nat} {n : nat} : n > foldr max 0 l → n ∉ l :=
-begin
-  induction l with m ms ih,
-  { simp },
-  { simp,
-    intros hm hn,
-    exact not_or_distrib.mpr (and.intro (ne_of_gt hm) (ih hn)) }
-end
-
-theorem exists_not_mem_of_gt_max {f : α → nat} (hf : bijective f) {l : list α} :
-  ∀ {n : nat}, n > foldr max 0 (map f l) → ∃ (a : α), f a = n ∧ a ∉ l :=
-begin
-  intros n hn,
-  rcases (bijective_iff_exists_unique f).mp hf n with ⟨b, hb, _⟩,
-  use b,
-  split,
-  { simp [hb] },
-  { have := not_mem_of_gt_max hn,
-    revert this,
-    contrapose,
-    simp,
-    intro h,
-    use [b, h, hb] }
-end
-
--- A simple nat result - can be tightened up, but how?
-theorem ne_of_add_eq_of_gt_zero {a b c : nat} : a > 0 → a + b = c → b ≠ c :=
-begin
-  intros ha habc hbc,
-  rw hbc at habc,
-  have : a + c > c, from lt_add_of_pos_left c ha,
-  rw habc at this,
-  exact nat.lt_asymm this this,
-end
-
--- Maximum values that map to general α
-theorem infimum_gt_list {f : nat → α} (f_inj : injective f) (l : list α) :
-  ∃ (n : nat), ∀ (m : nat), m ≥ n → f m ∉ l :=
-begin
-  induction l with a as ih,
-  { simp [not_mem_nil] },
-  { rcases ih with ⟨n, hn⟩,
-    by_cases h : ∃ (b : nat), f b = a,
-    { rcases h with ⟨b, hb⟩,
-      by_cases hnb : n > b,
-      { use n, 
-        intros m hm,
-        apply not_mem_cons_of_ne_of_not_mem,
-        { rw ← hb,
-          exact (injective.ne_iff f_inj).mpr (ne_of_gt (gt_of_ge_of_gt hm hnb)) },
-        { exact hn m hm } },
-      { use b + 1,
-        intros m hm,
-        simp at hnb,
-        apply not_mem_cons_of_ne_of_not_mem,
-        { rw ← hb,
-          exact (injective.ne_iff f_inj).mpr (ne_of_gt (nat.succ_le_iff.mp hm)) },
-        { exact hn m (le_trans hnb (nat.le_of_succ_le hm)) } } },
-    { simp at h,
-      use n,
-      intros m hm,
-      apply not_mem_cons_of_ne_of_not_mem,
-      { exact h m },
-      { exact hn m hm } } }
-end
-
-@[simp] theorem nil_inter [decidable_eq α] (l : list α) : l ∩ [] = [] :=
-eq_nil_of_subset_nil (inter_subset_right l [])
-
-theorem zero_left_of_add_zero {n m : nat} : 0 = n + m → n = 0 :=
-begin
-  cases m,
-  { rw add_zero n, intro h, exact h.symm },
-  { intro h, linarith }
-end
-
-theorem zero_right_of_add_zero {n m : nat} : 0 = n + m → m = 0 :=
-begin
-  cases n,
-  { rw zero_add m, intro h, exact h.symm },
-  { intro h, linarith }
-end
-
-theorem mem_fst_map_of_mem {l : list (α × β)} {a : α} {b : β} :
-  (a, b) ∈ l → a ∈ map prod.fst l :=
-begin
-  intro h,
-  apply mem_map.mpr,
-  use [(a, b), h]
-end
-
-theorem mem_snd_map_of_mem {l : list (α × β)} {a : α} {b : β} :
-  (a, b) ∈ l → b ∈ map prod.snd l :=
-begin
-  intro h,
-  apply mem_map.mpr,
-  use [(a, b), h]
-end
+theorem ne_tail_of_eq_head_of_ne [decidable_eq α] {a b : α} {l₁ l₂ : list α} :
+  (a :: l₁) ≠ (b :: l₂) → a = b → l₁ ≠ l₂ :=
+assume hne hab hl, absurd (congr (congr_arg cons hab) hl) hne
 
 theorem length_lt_length_cons (a : α) (l : list α) :
   length l < length (a :: l) :=
-by simp [length]
+by { rw length_cons, exact lt_add_one _ }
 
 theorem strong_induction_on_lists [inhabited α] {p : list α → Prop} (l : list α)
   (h : ∀ l₁, (∀ l₂, length l₂ < length l₁ → p l₂) → p l₁) : p l :=
@@ -289,10 +80,133 @@ suffices ∀ (l₁ : list α) (l₂ : list α), length l₂ < length l₁ → p 
   from this ((arbitrary α) :: l) l (length_lt_length_cons (arbitrary α) l),
 begin
   intro l₁, induction l₁ with a as ih,
-  { intros l₂ h₁, unfold length at h₁, exact absurd h₁ (l₂.length).not_lt_zero },
+  { intros l₂ h₁, exact absurd h₁ (l₂.length).not_lt_zero },
   { intros m h₁,
-    unfold length at h₁,
     apply or.by_cases (decidable.lt_or_eq_of_le (nat.le_of_lt_succ h₁)),
     { intros, apply ih, assumption },
     { intro hlen, have := h m, rw hlen at this, exact this ih } }
 end
+
+/- fold -/
+
+theorem foldr_bor_tt (l : list α) (f : α → bool) : 
+  foldr (λ x b, b || f x) tt l = tt :=
+begin
+  induction l with x xs ih,
+  { rw foldr_nil },
+  { rw [foldr_cons, ih, tt_bor] }
+end
+
+theorem foldr_band_ff (l : list α) (f : α → bool) :
+  foldr (λ x b, b && f x) ff l = ff :=
+begin
+  induction l with x xs ih,
+  { rw foldr_nil },
+  { rw [foldr_cons, ih, ff_band] }
+end
+
+section map
+
+variables {f : α → β} {a : α} {b : β} {l : list α}
+
+theorem exists_of_map_singleton : map f l = [b] → ∃ a, [a] = l ∧ f a = b :=
+begin
+  cases l with x xs,
+  { contradiction },
+  { simp [map_cons],
+    intros h₁ h₂,
+    simp [h₁, h₂] }
+end
+
+theorem exists_cons_of_map_cons {bs : list β} :
+  map f l = b :: bs → ∃ h L, l = h :: L ∧ f h = b ∧ map f L = bs :=
+begin
+  cases l with x xs,
+  { contradiction },
+  { rw map_cons,
+    intro h,
+    use [x, xs, ⟨refl _, (head_eq_of_cons_eq h), (tail_eq_of_cons_eq h)⟩] }
+end
+
+theorem exists_map_cons_of_map_cons {as : list α} : map f l = map f (a :: as) → 
+  ∃ h L, l = h :: L ∧ f h = f a ∧ map f L = map f as :=
+by { rw [map_cons], intro h, exact exists_cons_of_map_cons h }
+
+theorem mem_map_append {l₁ l₂ : list α} {f : α → β} {b : β} :
+  b ∈ map f (l₁ ++ l₂) → b ∈ map f l₁ ∨ b ∈ map f l₂ :=
+by { rw [map_append, mem_append], exact id }
+
+theorem mem_map_fst_of_mem {l : list (α × β)} {a : α} {b : β} :
+  (a, b) ∈ l → a ∈ map prod.fst l :=
+assume h, mem_map.mpr ⟨⟨a, b⟩, h, rfl⟩
+
+theorem mem_map_snd_of_mem {l : list (α × β)} {a : α} {b : β} :
+  (a, b) ∈ l → b ∈ map prod.snd l :=
+assume h, mem_map.mpr ⟨⟨a, b⟩, h, rfl⟩
+
+end map
+
+/- filter -/
+
+theorem length_filter {p : α → Prop} [decidable_pred p] {l : list α} : 
+  length (filter p l) ≤ length l :=
+begin
+  induction l with x xs ih,
+  { refl },
+  { by_cases p x,
+    { rw [filter_cons_of_pos _ h, length_cons, length_cons],
+      exact nat.succ_le_succ_iff.mpr ih },
+    { rw [filter_cons_of_neg _ h, length_cons],
+      exact le_add_right ih } }
+end
+
+/-! # Naturals and successors of supremums -/
+
+section nat
+
+open nat
+
+variables {f : α → nat} {l : list nat} {n m : nat}
+
+section max_nat
+
+def max_nat : list nat → nat
+| []        := 0
+| (n :: ns) := max n (max_nat ns)
+
+theorem max_nat_eq_foldr_max (l) : max_nat l = foldr max 0 l :=
+begin
+  induction l with n ns ih,
+  { refl },
+  { unfold max_nat, rw [foldr_cons, ih] }
+end
+
+theorem le_max_nat_of_mem : n ∈ l → n ≤ max_nat l :=
+begin
+  induction l with m ms ih,
+  { intro h, exact absurd h (not_mem_nil _) },
+  { intros h,
+    rcases eq_or_mem_of_mem_cons h with rfl | hms,
+    { exact le_max_iff.mpr (or.inl (le_refl n)) },
+    { exact le_max_iff.mpr (or.inr (ih hms)) } }
+end
+
+theorem not_mem_of_gt_max_nat : n > max_nat l → n ∉ l :=
+by { contrapose, simp, exact le_max_nat_of_mem }
+
+theorem exists_not_mem_of_bijective_of_gt_max_nat 
+  (hf : bijective f) {l : list α} :
+  n > max_nat (map f l) → ∃ a, f a = n ∧ a ∉ l :=
+begin
+  intros h,
+  rcases (bijective_iff_exists_unique f).mp hf n with ⟨b, hb, _⟩,
+  use b,
+  split,
+  { exact hb },
+  { intro hbl,
+    exact (not_mem_of_gt_max_nat h) (hb ▸ mem_map_of_mem f hbl) }
+end
+
+end max_nat
+
+end nat
