src/deprecated/xor.lean
@@ -1,0 +1,490 @@
+/-
+
+  This file concerns the definition and translation of XOR gates into CNF, and
+  proves that this translation is correct.
+
+  Authors: Cayden Codel, Jeremy Avigad, Marijn Heule
+  Carnegie Mellon University
+
+-/
+
+import data.bool
+import data.list.basic
+
+import cnf.literal
+import cnf.clause
+import cnf.cnf
+import cnf.explode
+import basic
+
+open list
+open literal
+open clause
+open cnf
+open explode
+
+/- An n-literal XOR gate is a list of those literals -/
+def xor_gate := list literal
+
+namespace xor_gate
+
+instance : has_append xor_gate := ⟨list.append⟩
+
+-- The conversion of the XOR gate to a clause is a nice way of sweeping
+-- uner the rug that the two definitions are actually identical
+-- TODO canonical way of saying we want the nil/empty clause?
+def to_clause (g : xor_gate) : clause :=
+  g.foldr (λ l c, l :: c) []
+
+-- Kinda cheesy
+lemma gate_eq_clause (g : xor_gate) : g = g.to_clause :=
+by simp [to_clause]
+
+/- Evaluates the XOR gate under an assignment -/
+def eval (α : assignment) (g : xor_gate) : bool :=
+  g.foldr (λ l b, b ⊕ l.eval α) ff
+
+def eval2 (α : assignment) (g : xor_gate) : bool :=
+  foldr bxor ff (map (literal.eval α) g)
+
+@[simp] theorem eval_nil (α : assignment) : eval α [] = ff := rfl
+
+theorem eval_cons (α : assignment) (l : literal) (g : xor_gate) : eval α (l :: g) = bxor (literal.eval α l) (eval α g) :=
+by simp [eval, foldr_cons, bool.bxor_comm]
+
+@[simp] theorem eval2_nil (α : assignment) : eval2 α [] = ff := rfl
+
+theorem eval2_cons (α : assignment) (l : literal) (g : xor_gate) : eval2 α (l :: g) = bxor (literal.eval α l) (eval2 α g) :=
+by simp [eval2, foldr_cons, bool.bxor_comm]
+
+theorem eval_eq_eval2 (α : assignment) (g : xor_gate) : eval α g = eval2 α g :=
+begin
+  induction g with l ls ih,
+  { simp },
+  { simp only [eval_cons, eval2_cons, ih] }
+end
+
+theorem eval_concat (α : assignment) (g₁ g₂ : xor_gate) : eval α (g₁ ++ g₂) = bxor (eval α g₁) (eval α g₂) :=
+begin
+  induction g₁ with l ls ih,
+  { simp },
+  { simp [eval_cons, ih] }
+end
+
+theorem eval_perm (α : assignment) {g₁ g₂ : xor_gate} :
+  g₁ ~ g₂ → eval α g₁ = eval α g₂ :=
+begin
+  intro h,
+  have : (map (literal.eval α) g₁) ~ (map (literal.eval α) g₂),
+  { exact perm.map (literal.eval α) h },
+  rw eval_eq_eval2,
+  rw eval_eq_eval2,
+  exact perm.foldr_eq (bool.bxor_left_comm) this ff
+end
+
+theorem eval_cons_conjunctive (α : assignment) (l : literal) (g : xor_gate) : 
+  eval α (l :: g) = (literal.eval α l || eval α g) && (!(literal.eval α l) || !(eval α g)) :=
+by simp only [← bxor_conjunctive, eval_cons α l g]
+
+theorem eval_cons_disjunctive (α : assignment) (l : literal) (g : xor_gate) :
+  eval α (l :: g) = (!(literal.eval α l) && eval α g) || (literal.eval α l && !(eval α g)) :=
+by simp only [← bxor_disjunctive, eval_cons α l g]
+
+/- Using a recursive evaluation function is sometimes more convenient -/
+def eval_rec (α : assignment) : xor_gate → bool
+| []        := ff
+| (l :: ls) := l.eval α ⊕ eval_rec ls
+
+/- To use the recursive definition, we need to prove that the two functions are equivalent -/
+theorem eval_and_eval_rec_equiv (α : assignment) (g : xor_gate) : eval α g = eval_rec α g :=
+begin
+  induction g with l ls ih,
+  { simp [eval_rec, eval] },
+  { simp [eval_rec, ih, eval_cons] },
+end
+
+/- The XOR gate evaluates to true if an odd number of literals evaluates to true -/
+theorem xor_odd_eval_tt (α : assignment) (g : xor_gate) : g.eval α = nat.bodd (g.countp (λ l, l.eval α = tt)) :=
+begin
+  induction g with l ls ih,
+  { simp },
+  { cases h : (l.eval α);
+    { simp [eval_cons, h, ih] } }
+end
+
+-- This is a shortcut of the above that uses gate.to_clause instead
+-- NOTE that the to_clause is essentially an identity operation, but if sets/permuations are
+-- used instead, the proof may grow more complex
+theorem xor_odd_eval_tt2 (α : assignment) (g : xor_gate) : g.eval α = nat.bodd (g.to_clause.count_tt α) :=
+begin
+  induction g with l ls ih,
+  { simp [to_clause] },
+  { cases h : (l.eval α);
+    { rw ← gate_eq_clause ls at ih,
+      simp [to_clause, eval_cons, count_tt_cons, bool.to_nat, h, ih] } }
+end
+
+/-! ## Naive encoding, simple version -/
+
+-- Let's start easier: turning a list of natural numbers into a cnf form
+-- The naive encoding returns a formula with all possible clauses with an even number of negated literals
+-- Because we are using natural numbers, i.e. positive literals, we want an even number of negative literals
+def nat_to_xor_cnf : list nat → cnf
+| []        := [[]]
+| (n :: ns) := (explode ns).map (λ c, cond (nat.bodd c.count_neg = ff) ((Pos n) :: c) ((Neg n) :: c))
+
+theorem mem_explode_of_mem_nat_to_xor :
+  ∀ {ns : list nat}, ∀ {c : clause}, c ∈ nat_to_xor_cnf ns → c ∈ explode ns
+| []        := by simp [nat_to_xor_cnf]
+| (n :: ns) := begin
+  simp [nat_to_xor_cnf, mem_map, mem_append],
+  intros c hc,
+  have : (Pos n).var = n ∧ (Neg n).var = n, simp [var], -- Make into literal lemma?
+  cases h : (c.count_neg.bodd);
+  { simp [h, this],
+    apply mem_explode_cons_of_mem_explode_of_lit,
+    exact hc }
+end
+
+theorem length_nat_to_xor_cnf : ∀ {ns : list nat}, ns ≠ [] → length (nat_to_xor_cnf ns) = 2^(length ns - 1)
+| []        := by { contradiction }
+| (n :: ns) := by simp [nat_to_xor_cnf, length_explode]
+
+theorem length_nat_to_xor_cnf_pos : ∀ {ns : list nat}, ns ≠ [] → length (nat_to_xor_cnf ns) > 0
+| []        := by { contradiction }
+| (n :: ns) := by simp [length_nat_to_xor_cnf]
+
+theorem exists_mem_nat_to_xor_of_ne_nil {ns : list nat} : ns ≠ [] → ∃ (c : clause), c ∈ nat_to_xor_cnf ns :=
+assume h, exists_mem_of_length_pos (length_nat_to_xor_cnf_pos h)
+
+theorem map_var_eq_of_mem_nat_to_xor : ∀ {ns : list nat}, ∀ {c : clause}, c ∈ nat_to_xor_cnf ns → c.map var = ns
+| []        := by simp [nat_to_xor_cnf]
+| (n :: ns) := begin
+  simp [nat_to_xor_cnf],
+  intros c hc,
+  cases h : c.count_neg.bodd;
+  { simp [h, var, map_var_eq_of_mem_explode hc] }
+end
+
+theorem mem_nat_to_xor_of_even_negation_of_map_var_eq : ∀ {ns : list nat}, ∀ {c : clause}, 
+  c.map var = ns → (nat.bodd c.count_neg = ff) → c ∈ nat_to_xor_cnf ns
+| []        := by simp [nat_to_xor_cnf]
+| (n :: ns) := begin
+  intros c hc,
+  rcases exists_cons_of_map_cons hc with ⟨l, ls, rfl, hl, hls⟩,
+  rcases pos_or_neg_of_var_eq_nat hl with rfl | rfl;
+  { simp [count_neg_cons, is_neg, bool.to_nat, nat_to_xor_cnf],
+    intro hcount, use ls,
+    simp [hcount, mem_explode_of_map_var_eq hls] }
+end
+
+theorem even_negation_of_mem_nat_to_xor_of_map_var_eq : ∀ {ns : list nat}, ∀ {c : clause}, 
+  c.map var = ns → c ∈ nat_to_xor_cnf ns → nat.bodd c.count_neg = ff
+| []        := by simp
+| (n :: ns) := begin
+  intros c hc hxor,
+  simp [nat_to_xor_cnf] at hxor,
+  rcases hxor with ⟨a, ha, hacons⟩,
+  rcases exists_cons_of_map_cons hc with ⟨l, ls, rfl, hl, hls⟩,
+  cases h : a.count_neg.bodd;
+  { simp [h] at hacons,
+    simp [← hacons, count_neg_cons, is_neg, bool.to_nat, h] },
+end
+
+theorem even_negation_iff_mem_nat_to_xor {ns : list nat} {c : clause} (hc : c.map var = ns) :
+  c ∈ nat_to_xor_cnf ns ↔ nat.bodd c.count_neg = ff :=
+⟨even_negation_of_mem_nat_to_xor_of_map_var_eq hc,
+  mem_nat_to_xor_of_even_negation_of_map_var_eq hc⟩
+
+theorem not_mem_nat_to_xor_cnf_of_odd_negation_of_map_var_eq {ns : list nat} {c : clause} :
+  c.map var = ns → (nat.bodd c.count_neg = tt) → c ∉ nat_to_xor_cnf ns :=
+begin
+  intros hc hcount,
+  by_contradiction,
+  exact absurd_bool hcount (even_negation_of_mem_nat_to_xor_of_map_var_eq hc h)
+end
+
+-- TODO move the c.map var assumption into the ns list nat portion since the above need it too
+theorem odd_negation_of_not_mem_nat_to_xor_of_map_var_eq {ns : list nat} {c : clause} (hc : c.map var = ns) :
+  c ∉ nat_to_xor_cnf ns → nat.bodd c.count_neg = tt :=
+begin
+  contrapose,
+  simp,
+  exact (even_negation_iff_mem_nat_to_xor hc).mpr
+end
+
+theorem odd_negation_iff_not_mem_nat_to_xor {ns : list nat} {c : clause} (hc : c.map var = ns) :
+  c ∉ nat_to_xor_cnf ns ↔ nat.bodd c.count_neg = tt :=
+⟨odd_negation_of_not_mem_nat_to_xor_of_map_var_eq hc, 
+  not_mem_nat_to_xor_cnf_of_odd_negation_of_map_var_eq hc⟩
+
+-- We prove that the naive encoding is equivalent to an XOR gate of all positive literals
+theorem nat_to_xor_cnf_correct (α : assignment) : ∀ (ns : list nat), 
+  cnf.eval α (nat_to_xor_cnf ns) = eval α (ns.map Pos)
+| []        := by simp [nat_to_xor_cnf]
+| (n :: ns) := begin
+  have red := xor_odd_eval_tt2 α (map Pos (n :: ns)),
+  cases h : (eval α (map Pos (n :: ns)));
+  rw [h, ← gate_eq_clause (map Pos (n :: ns))] at red,
+  -- ff case: We generate a false clause and show it is in the encoded formula
+  { apply eval_ff_iff_exists_clause_eval_ff.mpr,
+    use (falsify α (n :: ns)),
+    split,
+    { apply (even_negation_iff_mem_nat_to_xor (map_var_falsify_eq_list α (n :: ns))).mpr,
+      have oddeq := congr_arg nat.bodd (count_tt_pos_eq_count_neg_falsify α (n :: ns)),
+      rw ← red at oddeq,
+      exact oddeq.symm },
+    { exact falsify_eval_ff α (n :: ns) } },
+  -- tt case: Parities of α and clause tt evals means all clauses are true
+  { apply eval_tt_iff_forall_clause_eval_tt.mpr,
+    intros c hc,
+    have mve := map_var_eq_of_mem_nat_to_xor hc,
+    have neq := neq_of_ff_of_tt (eq.symm red) ((even_negation_iff_mem_nat_to_xor mve).mp hc),
+    exact eval_tt_of_opposite_parity (cons_ne_nil n ns) mve neq }
+end
+
+/-! # More complex encoding -/
+
+/-
+The above encoding assumed that the list of interest were only positive literals.
+Here, we generalize and prove the encoding valid with general lists of literals.
+The encoding is generated by counting "flips" between clauses rather than negations of literals.
+-/
+def xor_cnf : list literal → cnf
+| []        := [[]]
+| (l :: ls) := (explode (map var ls)).map (λ c, cond (nat.bodd (c.count_flips (ls)) = ff) (l :: c) (l.flip :: c))
+
+@[simp] theorem xor_cnf_singleton (l : literal) : xor_cnf [l] = [[l]] :=
+by simp [xor_cnf]
+
+theorem mem_explode_of_mem_xor_cnf :
+  ∀ {ls : list literal} {c : clause}, c ∈ xor_cnf ls → c ∈ explode (map var ls)
+| []        := by simp [xor_cnf]
+| (l :: ls) := begin
+  simp [xor_cnf, explode],
+  intros c hc,
+  cases l,
+  { cases h : (nat.bodd (c.count_flips ls)),
+    { use c, simp [h, hc, var, literal.flip] },
+    { right, use c, simp [h, hc, var, literal.flip] } },
+  { cases h : (nat.bodd (c.count_flips ls)), 
+    { right, use c, simp [h, hc, var, literal.flip] },
+    { use c, simp [h, hc, var, literal.flip] } }
+end
+
+theorem length_xor_cnf : ∀ {ls : list literal}, ls ≠ [] → length (xor_cnf ls) = 2^(length ls - 1)
+| []        := by { contradiction }
+| (l :: ls) := by simp [xor_cnf, length_explode]
+
+theorem length_xor_cnf_pos : ∀ {ls : list literal}, ls ≠ [] → length (xor_cnf ls) > 0
+| []        := by { contradiction }
+| (l :: ls) := by simp [length_xor_cnf]
+
+theorem exists_mem_xor_cnf_of_ne_nil {ls : list literal} : ls ≠ [] → ∃ (c : clause), c ∈ xor_cnf ls :=
+assume h, exists_mem_of_length_pos (length_xor_cnf_pos h)
+
+theorem map_var_eq_of_mem_xor_cnf {ls : list literal} : ∀ {c : clause}, c ∈ xor_cnf ls → map var c = map var ls :=
+begin
+  induction ls with l ls ih,
+  { simp [xor_cnf] },
+  { simp [xor_cnf],
+    intros c hc,
+    cases h : (nat.bodd (c.count_flips ls));
+    { simp [h, map_var_eq_of_mem_explode hc, flip_var_eq l] } }
+end
+
+-- TODO choose to add back in lemmas on flips for literal
+theorem mem_xor_cnf_of_even_flips_of_map_var_eq : ∀ {ls : list literal}, ∀ {c : clause},
+  map var c = map var ls → (nat.bodd (c.count_flips ls) = ff) → c ∈ xor_cnf ls
+| []        := by simp [xor_cnf]
+| (l :: ls) := begin
+  simp [xor_cnf, map_cons],
+  intros c hc hcount,
+  rcases exists_cons_of_map_cons hc with ⟨d, ds, rfl, hd, hds⟩,
+  use ds,
+  cases htf : (nat.bodd (count_flips ds ls)),
+  { by_cases l.flip = d,
+    { have : d.flip = l, from congr_arg literal.flip h ▸ flip_flip l,
+      simp [count_flips, this] at hcount,
+      exact absurd_bool hcount htf },
+    { simp [htf, mem_explode_of_map_var_eq hds, hd], --eq_of_flip_ne_of_var_eq hd.symm h]
+      rcases eq_or_flip_eq_of_var_eq hd with rfl | h₂,
+      { refl },
+      { have : d = l.flip, from congr_arg literal.flip h₂ ▸ (flip_flip d).symm, 
+        exact absurd this (ne.symm h) } } },
+  { by_cases l.flip = d,
+    { simp [htf, mem_explode_of_map_var_eq hds, hd, h], },
+    { have := function.injective.ne flip_injective h,
+      rw flip_flip at this,
+      simp [count_flips, ne.symm this] at hcount,
+      exact absurd_bool htf hcount } }
+end
+
+theorem even_flips_of_mem_xor_cnf_of_map_var_eq : ∀ {ls : list literal}, ∀ {c : clause},
+  c.map var = map var ls → c ∈ xor_cnf ls → nat.bodd (count_flips c ls) = ff
+| []        := by simp [xor_cnf]
+| (l :: ls) := begin
+  intros c hc hxor,
+  simp [xor_cnf] at hxor,
+  rcases hxor with ⟨a, ha, hacons⟩,
+  rcases exists_cons_of_map_cons hc with ⟨c, cs, rfl, hc2, hcs⟩,
+  cases h : (nat.bodd (count_flips a ls));
+  { simp [h] at hacons,
+    simp [← hacons, count_flips, is_neg, bool.to_nat, h, flip_flip _, flip_ne] }
+end
+
+theorem even_flips_iff_mem_xor_cnf {ls : list literal} {c : clause} (hc : c.map var = map var ls) :
+  nat.bodd (count_flips c ls) = ff ↔ c ∈ xor_cnf ls :=
+⟨mem_xor_cnf_of_even_flips_of_map_var_eq hc, even_flips_of_mem_xor_cnf_of_map_var_eq hc⟩
+
+theorem not_mem_xor_cnf_of_odd_flips_of_map_var_eq {ls : list literal} {c : clause} :
+  map var c = map var ls → (nat.bodd (count_flips c ls)) = tt → c ∉ xor_cnf ls :=
+begin
+  intros hc hcount,
+  by_contradiction,
+  exact absurd_bool hcount ((even_flips_iff_mem_xor_cnf hc).mpr h)
+end
+
+theorem odd_flips_of_not_mem_xor_cnf_of_map_var_eq {ls : list literal} {c : clause} :
+  map var c = map var ls → c ∉ xor_cnf ls → (nat.bodd (count_flips c ls)) = tt :=
+begin
+  intro hc,
+  contrapose,
+  simp,
+  exact (even_flips_iff_mem_xor_cnf hc).mp
+end
+
+theorem odd_flips_iff_not_mem_xor_cnf {ls : list literal} {c : clause} (hc : map var c = map var ls) :
+  nat.bodd (count_flips c ls) = tt ↔ c ∉ xor_cnf ls :=
+⟨not_mem_xor_cnf_of_odd_flips_of_map_var_eq hc, odd_flips_of_not_mem_xor_cnf_of_map_var_eq hc⟩
+
+-- A restatement of the above theorem in a more general way
+-- Alternatively, the assignment can be manipulated by flipping the correct literals
+theorem xor_cnf_correct (α : assignment) : ∀ (ls : list literal),
+  cnf.eval α (xor_cnf ls) = eval α ls
+| []        := by simp [xor_cnf]
+| (l :: ls) := begin
+  have red := xor_odd_eval_tt2 α (l :: ls),
+  cases h : (eval α (l :: ls));
+  rw [h, ← gate_eq_clause (l :: ls)] at red,
+  { apply eval_ff_iff_exists_clause_eval_ff.mpr,
+    use (falsify α (map var (l :: ls))),
+    split,
+    { rw ← count_flips_falsify_eq_count_tt α (l :: ls) at red,
+      rw count_flips_comm at red,
+      apply (even_flips_iff_mem_xor_cnf (map_var_falsify_eq_list α (map var (l :: ls)))).mp,
+      exact red.symm },
+    { exact falsify_eval_ff α (map var (l :: ls)) } },
+  { apply eval_tt_iff_forall_clause_eval_tt.mpr,
+    intros c hc,
+    have mve := map_var_eq_of_mem_xor_cnf hc,
+    have neqodd := neq_of_ff_of_tt (eq.symm red) ((even_flips_iff_mem_xor_cnf mve).mpr hc),
+    have neq := ne_of_apply_ne nat.bodd neqodd,
+    rw count_flips_comm at neq,
+    exact eval_tt_of_neq_flips (cons_ne_nil l ls) c mve.symm neq }
+end
+
+theorem vars_cnf_subset_xor {ls : list literal} :
+  ls ≠ [] → cnf.vars (xor_cnf ls) ⊆ (map var ls) :=
+begin
+  intro h,
+  cases ls,
+  { contradiction },
+  { intros n hn,
+    rcases cnf.exists_mem_clause_of_mem_vars hn with ⟨c, hcnf, hc⟩,
+    simp [← map_var_eq_of_mem_xor_cnf hcnf, mem_vars_iff_mem_map_vars, hc] }
+end
+
+end xor_gate
+
+/-! # Equivalence on domain for this encoding -/
+
+namespace assignment
+
+theorem equiv_on_domain_for_xor {α₁ α₂ : assignment} : ∀ {ls : list literal},
+  (α₁ ≡[map var ls]≡ α₂) → xor_gate.eval α₁ ls = xor_gate.eval α₂ ls :=
+begin
+  intros ls heq,
+  cases ls,
+  { simp },
+  { have := eqod_subset_of_eqod (xor_gate.vars_cnf_subset_xor (cons_ne_nil ls_hd ls_tl)) heq,
+    simp [← xor_gate.xor_cnf_correct α₁, 
+      ← xor_gate.xor_cnf_correct α₂, eval_eq_of_equiv_on_domain_vars this] }
+end
+
+end assignment
+
+namespace xor_gate
+
+theorem exists_assignment_eval_tt_of_nodup {l : list literal} :
+  l ≠ [] → nodup (map var l) → ∃ (α : assignment), eval α l = tt :=
+begin
+  induction l with l ls ih,
+  { simp },
+  { intros _ hnodup,
+    cases ls,
+    { cases l,
+      { use assignment.all_tt, simp [eval, literal.eval, assignment.all_tt_eval_tt] },
+      { use assignment.all_ff, simp [eval, literal.eval, assignment.all_ff_eval_ff] } },
+    { rw map_cons at hnodup,
+      rcases ih (cons_ne_nil _ _) (nodup_of_nodup_cons hnodup) with ⟨α, ha⟩,
+      cases l,
+      { have : (λ x, if x = l then ff else α x) ≡[map var (ls_hd :: ls_tl)]≡ α,
+        { intros x hx,
+          unfold var at hnodup,
+          have : l ∉ (map var (ls_hd :: ls_tl)), from not_mem_of_nodup_cons hnodup,
+          by_cases h : x = l,
+          { rw ← h at this, exact absurd hx this },
+          { simp [h] } },
+        use (λ x, if x = l then ff else α x),
+        rw xor_gate.eval_cons,
+        simp [literal.eval, assignment.equiv_on_domain_for_xor this, ha] },
+      { have : (λ x, if x = l then tt else α x) ≡[map var (ls_hd :: ls_tl)]≡ α,
+        { intros x hx,
+          unfold var at hnodup,
+          have : l ∉ (map var (ls_hd :: ls_tl)), from not_mem_of_nodup_cons hnodup,
+          by_cases h : x = l,
+          { rw ← h at this, exact absurd hx this },
+          { simp [h] } },
+        use (λ x, if x = l then tt else α x),
+        rw xor_gate.eval_cons,
+        simp [literal.eval, assignment.equiv_on_domain_for_xor this, ha] } } }
+end
+
+theorem exists_assignment_eval_ff_of_nodup {l : list literal} :
+  l ≠ [] → nodup (map var l) → ∃ (α : assignment), eval α l = ff :=
+begin
+  intros hnil hnodup,
+  rcases exists_cons_of_ne_nil hnil with ⟨l, ls, rfl⟩,
+  rw map_cons at hnodup,
+  cases ls,
+  { cases l, 
+    { use assignment.all_ff,
+      simp [eval, assignment.all_ff_eval_ff, literal.eval] },
+    { use assignment.all_tt,
+      simp [eval, assignment.all_tt_eval_tt, literal.eval] } },
+  { rcases exists_assignment_eval_tt_of_nodup (cons_ne_nil ls_hd ls_tl) (nodup_of_nodup_cons hnodup) with ⟨α, ha⟩,
+    cases l,
+    { use (λ x, if x = l then tt else α x),
+      have : (λ x, if x = l then tt else α x) ≡[map var (ls_hd :: ls_tl)]≡ α,
+      { intros x hx,
+          unfold var at hnodup,
+          have : l ∉ (map var (ls_hd :: ls_tl)), from not_mem_of_nodup_cons hnodup,
+          by_cases h : x = l,
+          { rw ← h at this, exact absurd hx this },
+          { simp [h] } },
+      rw eval_cons,
+      simp [literal.eval, assignment.equiv_on_domain_for_xor this, ha] },
+    { use (λ x, if x = l then ff else α x),
+      have : (λ x, if x = l then ff else α x) ≡[map var (ls_hd :: ls_tl)]≡ α,
+      { intros x hx,
+          unfold var at hnodup,
+          have : l ∉ (map var (ls_hd :: ls_tl)), from not_mem_of_nodup_cons hnodup,
+          by_cases h : x = l,
+          { rw ← h at this, exact absurd hx this },
+          { simp [h] } },
+      rw eval_cons,
+      simp [literal.eval, assignment.equiv_on_domain_for_xor this, ha] } }
+end
+
+end xor_gate
