src/xor/direct_xor.lean
@@ -1,0 +1,227 @@
+/-
+This file defines and proves the equisatisfiability of the direct (or naive)
+encoding for the n-variable XOR gate.
+
+Authors: Cayden Codel, Jeremy Avigad, Marijn Heule
+Carnegie Mellon University
+-/
+
+import cnf.literal
+import cnf.assignment
+import cnf.clause
+import cnf.cnf
+import xor.xor
+import basic
+
+import data.list.basic
+import data.nat.basic
+
+universe u
+
+-- Represents the parametric type of the variable stored in the literal
+variables {V : Type u} [decidable_eq V] [inhabited V]
+
+namespace xor_gate
+
+open literal
+open clause
+open cnf
+open list
+open xor_gate
+open explode
+open nat
+
+/-! # Direct encoding -/
+section direct_encoding
+
+variables {g : xor_gate V} {c : clause V}
+
+/- The direct encoding is the set of all possible clauses with an even number 
+   of negations on the provided literals in a single CNF formula. -/
+def direct_xor : xor_gate V → cnf V
+| []        := [[]]
+| (l :: ls) := (explode (map var ls)).map 
+      (λ c, cond (bodd (c.count_flips (ls)) = ff) (l :: c) (l.flip :: c))
+
+@[simp] theorem direct_xor_nil : direct_xor ([] : xor_gate V) = [[]] := rfl
+
+@[simp] theorem direct_xor_singleton (l : literal V) : direct_xor [l] = [[l]] :=
+by simp [direct_xor]
+
+theorem mem_explode_of_mem_direct_xor : 
+  c ∈ direct_xor g → c ∈ explode (map var g) :=
+begin
+  cases g with l ls,
+  { simp only [explode_nil, imp_self, direct_xor_nil, map_nil] },
+  { simp [direct_xor, explode],
+    intros cl hcl,
+    cases l,
+    { cases (bodd (cl.count_flips ls)),
+      { simp, intro h, use [cl, hcl, h] },
+      { simp, intro h, unfold literal.flip at h, 
+        right, use [cl, hcl, h] } },
+    { cases (bodd (cl.count_flips ls)),
+      { simp, intro h, right, use [cl, hcl, h] },
+      { simp, intro h, unfold literal.flip at h,
+        use [cl, hcl, h] } } }
+end
+
+theorem length_direct_xor : g ≠ [] → length (direct_xor g) = 2^(length g - 1) :=
+begin
+  cases g,
+  { contradiction },
+  { simp only [direct_xor, length_explode, add_zero, length, add_succ_sub_one, 
+      ne.def, forall_true_left, not_false_iff, length_map] }
+end
+
+theorem length_direct_xor_pos : g ≠ [] → length (direct_xor g) > 0 :=
+assume h, by simp only [length_direct_xor h, succ_pos', gt_iff_lt, pow_pos]
+
+theorem exists_mem_direct_xor (g : xor_gate V) : 
+  ∃ (c : clause V), c ∈ direct_xor g :=
+begin
+  cases g with l ls,
+  { use [nil, mem_singleton_self nil] },
+  { exact exists_mem_of_length_pos (length_direct_xor_pos (cons_ne_nil l ls)) }
+end
+
+-- These theorems begin to be dependent on order of encoding
+-- If the underlying type of xor_gate changes to (fin)set, must update
+theorem map_var_eq_of_mem_direct_xor :
+  c ∈ direct_xor g → map var c = map var g :=
+begin
+  cases g with l ls,
+  { simp only [direct_xor, imp_self, map_eq_nil, map_nil, mem_singleton] },
+  { simp [direct_xor],
+    intros c hc,
+    cases (bodd (c.count_flips ls)),
+    { simp only [if_true, eq_self_iff_true],
+      rintro rfl,
+      simp [map_var_eq_iff_mem_explode.mpr hc] },
+    { simp only [if_false],
+      rintro rfl,
+      simp [map_var_eq_iff_mem_explode.mpr hc, flip_var_eq] } }
+end
+
+theorem even_flips_iff_mem_direct_xor_of_map_var_eq : map var c = map var g → 
+  (bodd (c.count_flips g) = ff ↔ c ∈ direct_xor g) :=
+begin
+  intro hc, split,
+  { cases g with l ls,
+    { revert hc, simp },
+    { simp only [direct_xor, map_cons, bool.cond_to_bool, mem_map],
+      intro hf,
+      rcases exists_cons_of_map_cons hc with ⟨x, xs, rfl, hx, hxs⟩,
+      use xs, split,
+      { exact map_var_eq_iff_mem_explode.mp hxs },
+      { cases h : (bodd (clause.count_flips xs ls)),
+        { rcases var_eq_iff_eq_or_flip_eq.mp hx with rfl | hx,
+          { simp only [if_true, eq_self_iff_true] },
+          { simp [clause.count_flips, hx] at hf,
+            rw h at hf, contradiction } },
+        { rcases var_eq_iff_eq_or_flip_eq.mp hx with hx | rfl,
+          { simp [clause.count_flips, hx] at hf,
+            rw h at hf, contradiction },
+          { simp only [flip_flip, if_false] } } } } },
+  { cases g with l ls,
+    { simp },
+    { simp only [direct_xor, bool.cond_to_bool, mem_map],
+      rintro ⟨a, ha, hf⟩,
+      rcases exists_cons_of_map_cons hc with ⟨x, xs, rfl, hx, hxs⟩,
+      cases h : (nat.bodd (a.count_flips ls));
+      { simp only [h, if_true, eq_self_iff_true, if_false] at hf,
+        simp [← hf, clause.count_flips, literal.is_neg, 
+          bool.to_nat, h, flip_flip _, flip_ne] } } }      
+end
+
+theorem odd_flips_iff_not_mem_direct_xor_of_map_var_eq : map var c = map var g → 
+  (bodd (c.count_flips g) = tt ↔ c ∉ direct_xor g) :=
+begin
+  intro hc, split,
+  { intro hcount, by_contradiction,
+    rw (even_flips_iff_mem_direct_xor_of_map_var_eq hc).mpr h at hcount,
+    contradiction },
+  { contrapose, simp only [eq_ff_eq_not_eq_tt, not_not],
+    exact (even_flips_iff_mem_direct_xor_of_map_var_eq hc).mp }
+end
+
+theorem direct_xor_equisatisfiable (g : xor_gate V) :
+  assignment.eqsat (λ α, cnf.eval α (direct_xor g)) (λ α, g.eval α) :=
+begin
+  split,
+  { rintros ⟨α, ha⟩,
+    use α, simp [eval_eq_bodd_count_tt α g], simp at ha,
+    rcases exists_mem_direct_xor g with ⟨c, hc⟩,
+    by_contradiction,
+    rw eq_ff_eq_not_eq_tt at h,
+    --rw clause.count_tt_pos_eq_count_neg_falsify at h,
+    --have := eval_tt_iff_forall_clause_eval_tt.mp ha,
+    rw [← clause.count_flips_falsify_eq_count_tt, count_flips_comm] at h,
+    have falsify_mem := mem_direct_xor_of_even_flips_of_map_var_eq
+      (map_var_falsify_eq_list α (map var l)) h,
+  have falsify_eval := falsify_eval_ff α (map var l),
+  have := this (falsify α (map var l)) falsify_mem,
+  exact absurd_bool this falsify_eval
+  },
+  { rintros ⟨α, ha⟩,
+    rw xor_odd_eval_tt α g at ha,
+  rw ← gate_eq_clause l at ha,
+  use α,
+  apply eval_tt_iff_forall_clause_eval_tt.mpr,
+  intros c hc,
+  have mve := map_var_eq_of_mem_direct_xor hc,
+  have neqodd := neq_of_ff_of_tt ha ((even_flips_iff_mem_direct_xor mve).mpr hc),
+  have neq := ne_of_apply_ne nat.bodd neqodd,
+  rw count_flips_comm at neq,
+  exact eval_tt_of_neq_flips mve.symm neq
+
+    exact exists_xor_of_direct_xor ⟨α, ha⟩ }
+end
+
+-- Some proofs require that the naive encoding exactly represents xor. Equality is stronger
+-- Technically, equality is stronger than equisatisfiability, think about replacing above?
+theorem eval_direct_xor_eq_eval_xor_gate (l : list (literal V)) (α : assignment V) :
+  cnf.eval α (direct_xor l) = xor_gate.eval α l :=
+begin
+  cases l with l ls,
+  { simp },
+  { have red := xor_odd_eval_tt2 α (l :: ls),
+    cases h : (xor_gate.eval α (l :: ls));
+    rw [h, ← gate_eq_clause (l :: ls)] at red,
+    { apply eval_ff_iff_exists_clause_eval_ff.mpr,
+      use (falsify α (map var (l :: ls))),
+      split,
+      { rw ← count_flips_falsify_eq_count_tt α (l :: ls) at red,
+        rw count_flips_comm at red,
+        apply (even_flips_iff_mem_direct_xor (map_var_falsify_eq_list α (map var (l :: ls)))).mp,
+        exact red.symm },
+      { exact falsify_eval_ff α (map var (l :: ls)) } },
+    { apply eval_tt_iff_forall_clause_eval_tt.mpr,
+      intros c hc,
+      have mve := map_var_eq_of_mem_direct_xor hc,
+      have neqodd := neq_of_ff_of_tt (eq.symm red) ((even_flips_iff_mem_direct_xor mve).mpr hc),
+      have neq := ne_of_apply_ne nat.bodd neqodd,
+      rw count_flips_comm at neq,
+      exact eval_tt_of_neq_flips mve.symm neq }
+  }
+end
+
+theorem vars_cnf_subset_xor {ls : list (literal V)} :
+  ls ≠ [] → cnf.vars (direct_xor ls) ⊆ (map var ls) :=
+begin
+  intro h,
+  cases ls,
+  { contradiction },
+  { intros n hn,
+    rcases cnf.exists_mem_clause_of_mem_vars hn with ⟨c, hcnf, hc⟩,
+    simp [← map_var_eq_of_mem_direct_xor hcnf, mem_vars_iff_mem_map_vars, hc] }
+end
+
+theorem vars_direct_xor_subset_vars {l : list (literal V)} :
+  l ≠ [] → cnf.vars (direct_xor l) ⊆ clause.vars l :=
+assume h, subset.trans (vars_cnf_subset_xor h) (map_var_subset_of_vars l)
+
+end direct_encoding
+
+end xor_gate
+
